src/Word/Interface.v
@@ -1,92 +1,116 @@
 (* Specification of two's complement machine words wrt Z *)
 
-Require Import Coq.ZArith.BinIntDef Coq.ZArith.BinInt.
+Require Import Coq.ZArith.BinIntDef Coq.ZArith.BinInt Coq.ZArith.Zdigits.
 Local Open Scope Z_scope.
 
 Module word.
   Class word {width : Z} := {
-    rep : Type;
+                             rep : Type;
 
-    (* defining relations *)
-    unsigned : rep -> Z;
-    signed : rep -> Z;
-    of_Z : Z -> rep;
+                             (* defining relations *)
+                             unsigned : rep -> Z;
+                             signed : rep -> Z;
+                             of_Z : Z -> rep;
+                             of_bool : bool -> rep;
+                             max_word : rep;
+                             min_word : rep;
 
-    (* operations *)
-    add : rep -> rep -> rep;
-    sub : rep -> rep -> rep;
-    opp : rep -> rep;
+                             (* operations *)
+                             add : rep -> rep -> rep;
+                             sub : rep -> rep -> rep;
+                             opp : rep -> rep;
 
-    or : rep -> rep -> rep;
-    and : rep -> rep -> rep;
-    xor : rep -> rep -> rep;
-    not : rep -> rep;
-    ndn : rep -> rep -> rep;
+                             or : rep -> rep -> rep;
+                             and : rep -> rep -> rep;
+                             xor : rep -> rep -> rep;
+                             not : rep -> rep;
+                             ndn : rep -> rep -> rep;
+                             uand : rep -> rep;
+                             uor : rep -> rep;
+                             uxor : rep -> rep;
 
-    mul : rep -> rep -> rep;
-    mulhss : rep -> rep -> rep;
-    mulhsu : rep -> rep -> rep;
-    mulhuu : rep -> rep -> rep;
+                             mul : rep -> rep -> rep;
+                             mulhss : rep -> rep -> rep;
+                             mulhsu : rep -> rep -> rep;
+                             mulhuu : rep -> rep -> rep;
 
-    divu : rep -> rep -> rep;
-    divs : rep -> rep -> rep; (* Z.quot *)
-    modu : rep -> rep -> rep;
-    mods : rep -> rep -> rep; (* Z.rem *)
+                             divu : rep -> rep -> rep;
+                             divs : rep -> rep -> rep; (* Z.quot *)
+                             modu : rep -> rep -> rep;
+                             mods : rep -> rep -> rep; (* Z.rem *)
 
-    slu : rep -> rep -> rep;
-    sru : rep -> rep -> rep;
-    srs : rep -> rep -> rep;
+                             slu : rep -> rep -> rep;
+                             sru : rep -> rep -> rep;
+                             srs : rep -> rep -> rep;
 
-    eqb : rep -> rep -> bool;
-    ltu : rep -> rep -> bool;
-    lts : rep -> rep -> bool;
+                             eqb : rep -> rep -> bool;
+                             ltu : rep -> rep -> bool;
+                             lts : rep -> rep -> bool;
 
-    gtu x y := ltu y x;
-    gts x y := lts y x;
+                             gtu x y := ltu y x;
+                             gts x y := lts y x;
 
-    swrap z := (z + 2^(width-1)) mod 2^width - 2^(width-1);
+                             swrap z := (z + 2^(width-1)) mod 2^width - 2^(width-1);
 
-    sextend: Z -> rep -> rep; (* Z is bitwidth of input *)
-  }.
+                             sextend: Z -> rep -> rep; (* Z is bitwidth of input *)
+                           }.
+
+
   Arguments word : clear implicits.
+  
 
   Class ok {width} {word : word width}: Prop := {
-    wrap z := z mod 2^width;
+                                                 wrap z := z mod 2^width;
 
-    width_pos: 0 < width;
+                                                 width_pos: 0 < width;
 
-    unsigned_of_Z : forall z, unsigned (of_Z z) = wrap z;
-    signed_of_Z : forall z, signed (of_Z z) = swrap z;
-    of_Z_unsigned : forall x, of_Z (unsigned x) = x;
+                                                 unsigned_of_Z : forall z, unsigned (of_Z z) = wrap z;
+                                                 signed_of_Z : forall z, signed (of_Z z) = swrap z;
+                                                 of_Z_unsigned : forall x, of_Z (unsigned x) = x;
+                                                 of_bool_unsigned : forall x, unsigned (of_bool x) = wrap (ZArith.Zdigits.bit_value x);
+                                                 max_word_unsigned : unsigned max_word = (wrap (-1)%Z);
+                                                 min_word_unsigned : unsigned min_word = (wrap 0%Z);
 
-    unsigned_add : forall x y, unsigned (add x y) = wrap (Z.add (unsigned x) (unsigned y));
-    unsigned_sub : forall x y, unsigned (sub x y) = wrap (Z.sub (unsigned x) (unsigned y));
-    unsigned_opp : forall x, unsigned (opp x) = wrap (Z.opp (unsigned x));
+                                                 unsigned_add : forall x y, unsigned (add x y) = wrap (Z.add (unsigned x) (unsigned y));
+                                                 unsigned_sub : forall x y, unsigned (sub x y) = wrap (Z.sub (unsigned x) (unsigned y));
+                                                 unsigned_opp : forall x, unsigned (opp x) = wrap (Z.opp (unsigned x));
 
-    unsigned_or : forall x y, unsigned (or x y) = wrap (Z.lor (unsigned x) (unsigned y));
-    unsigned_and : forall x y, unsigned (and x y) = wrap (Z.land (unsigned x) (unsigned y));
-    unsigned_xor : forall x y, unsigned (xor x y) = wrap (Z.lxor (unsigned x) (unsigned y));
-    unsigned_not : forall x, unsigned (not x) = wrap (Z.lnot (unsigned x));
-    unsigned_ndn : forall x y, unsigned (ndn x y) = wrap (Z.ldiff (unsigned x) (unsigned y));
+                                                 unsigned_or : forall x y, unsigned (or x y) = wrap (Z.lor (unsigned x) (unsigned y));
+                                                 unsigned_and : forall x y, unsigned (and x y) = wrap (Z.land (unsigned x) (unsigned y));
+                                                 unsigned_xor : forall x y, unsigned (xor x y) = wrap (Z.lxor (unsigned x) (unsigned y));
+                                                 unsigned_not : forall x, unsigned (not x) = wrap (Z.lnot (unsigned x));
+                                                 unsigned_ndn : forall x y, unsigned (ndn x y) = wrap (Z.ldiff (unsigned x) (unsigned y));
+                                                 unsigned_uand : forall x, unsigned (uand x) = wrap (ZArith.Zdigits.bit_value (Z.eqb ((wrap (-1)%Z)) (unsigned x)));
+                                                 unsigned_uor : forall x, unsigned (uor x) =  wrap (ZArith.Zdigits.bit_value (negb (Z.eqb ((wrap 0)) (unsigned x))));
+                                                 
 
-    unsigned_mul : forall x y, unsigned (mul x y) = wrap (Z.mul (unsigned x) (unsigned y));
-    signed_mulhss : forall x y, signed (mulhss x y) = swrap (Z.mul (signed x) (signed y) / 2^width);
-    signed_mulhsu : forall x y, signed (mulhsu x y) = swrap (Z.mul (signed x) (unsigned y) / 2^width);
-    unsigned_mulhuu : forall x y, unsigned (mulhuu x y) = wrap (Z.mul (unsigned x) (unsigned y) / 2^width);
+                                                 unsigned_mul : forall x y, unsigned (mul x y) = wrap (Z.mul (unsigned x) (unsigned y));
+                                                 signed_mulhss : forall x y, signed (mulhss x y) = swrap (Z.mul (signed x) (signed y) / 2^width);
+                                                 signed_mulhsu : forall x y, signed (mulhsu x y) = swrap (Z.mul (signed x) (unsigned y) / 2^width);
+                                                 unsigned_mulhuu : forall x y, unsigned (mulhuu x y) = wrap (Z.mul (unsigned x) (unsigned y) / 2^width);
 
-    unsigned_divu : forall x y, unsigned y <> 0 -> unsigned (divu x y) = wrap (Z.div (unsigned x) (unsigned y));
-    signed_divs : forall x y, signed y <> 0 -> signed x <> -2^(width-1) \/ signed y <> -1 -> signed (divs x y) = swrap (Z.quot (signed x) (signed y));
-    unsigned_modu : forall x y, unsigned y <> 0 -> unsigned (modu x y) = wrap (Z.modulo (unsigned x) (unsigned y));
-    signed_mods : forall x y, signed y <> 0 -> signed (mods x y) = swrap (Z.rem (signed x) (signed y));
+                                                 unsigned_divu : forall x y, unsigned y <> 0 -> unsigned (divu x y) = wrap (Z.div (unsigned x) (unsigned y));
+                                                 signed_divs : forall x y, signed y <> 0 -> signed x <> -2^(width-1) \/ signed y <> -1 -> signed (divs x y) = swrap (Z.quot (signed x) (signed y));
+                                                 unsigned_modu : forall x y, unsigned y <> 0 -> unsigned (modu x y) = wrap (Z.modulo (unsigned x) (unsigned y));
+                                                 signed_mods : forall x y, signed y <> 0 -> signed (mods x y) = swrap (Z.rem (signed x) (signed y));
 
-    unsigned_slu : forall x y, Z.lt (unsigned y) width -> unsigned (slu x y) = wrap (Z.shiftl (unsigned x) (unsigned y));
-    unsigned_sru : forall x y, Z.lt (unsigned y) width -> unsigned (sru x y) = wrap (Z.shiftr (unsigned x) (unsigned y));
-    signed_srs : forall x y, Z.lt (unsigned y) width -> signed (srs x y) = swrap (Z.shiftr (signed x) (unsigned y));
+                                                 unsigned_slu : forall x y, Z.lt (unsigned y) width -> unsigned (slu x y) = wrap (Z.shiftl (unsigned x) (unsigned y));
+                                                 unsigned_sru : forall x y, Z.lt (unsigned y) width -> unsigned (sru x y) = wrap (Z.shiftr (unsigned x) (unsigned y));
+                                                 signed_srs : forall x y, Z.lt (unsigned y) width -> signed (srs x y) = swrap (Z.shiftr (signed x) (unsigned y));
 
-    unsigned_eqb : forall x y, eqb x y = Z.eqb (unsigned x) (unsigned y);
-    unsigned_ltu : forall x y, ltu x y = Z.ltb (unsigned x) (unsigned y);
-    signed_lts : forall x y, lts x y = Z.ltb (signed x) (signed y);
-  }.
+                                                 unsigned_eqb : forall x y, eqb x y = Z.eqb (unsigned x) (unsigned y);
+                                                 unsigned_ltu : forall x y, ltu x y = Z.ltb (unsigned x) (unsigned y);
+                                                 signed_lts : forall x y, lts x y = Z.ltb (signed x) (signed y);
+                                               }.
+
+
   Arguments ok {_} _.
-End word. Notation word := word.word.
+
+  
+End word.
+
+Notation word := word.word.
+
 Global Coercion word.rep : word >-> Sortclass.
+
+
